\section*{Exercise 10}

Show that 

\[
	\genericmat{v}{
		1&x&x^2\\
		1&y&y^2\\
		1&z&z^2
	} =
	(z-x)(z-y)(y-z)
\]

Computing this determinant manually gives us:

\[
	z^2y + y^2x + x^2z - z^2x - y^2z - x^2y
\]

To see if these are equal to the above triple product we can expand that one out!

\[
	\begin{aligned}
		(z-x)(z-y)(y-z) &= z^2 - zy - zx + xy \\
		&= (y-x)(z^2 - zy - zx + xy) \\
		&= z^2y - zy^2 - zxy + xy^2 - z^2x + zxy + 2x^2 - x^2y \\
		&= z^2y + y^2x + x^2z - z^2x - y^2z - x^2y
	\end{aligned}
\]

Which is the same as what we manually computed above! 
