\section*{Exercise 3.3}
For each linear transformation below find its matrix.

\subsection*{Part A}
$T: \R^2 \to \R^3$ defined by:
\[T(x,y)^T = \genericmat{p}{x+2y\\2x-5y\\7y}\]

Same gameplan as 3.2, we transform our standard basis vectors and use those to get the matrix of the transformation.

\[
	\begin{aligned}
		T(\vec{e_1}) &= \genericmat{p}{1\\2\\0} \\
		T(\vec{e_2}) &= \genericmat{p}{2\\-5\\7}
	\end{aligned}
\]

From this we can state that the matrix of this transformation is:

\[A = \genericmat{p}{1&2\\2&-5\\0&7}\]

\subsection*{Part B}
$T: \R^4 \to \R^3$ defined by:

\[
	T \genericmat{p}{x_1\\x_2\\x_3\\x_3} = 
	\genericmat{p}
	{x_1+x_2+x_3+x_4 \\ 
	x_2 - x_4 \\ 
	x_1 + 3x_2 + 
	6x_4}
\]

\[
	\begin{aligned}
		T(\vec{e_1}) &= (1,0,1)^T \\
		T(\vec{e_2}) &= (1,1,3)^T \\
		T(\vec{e_3}) &= (1,0,0)^T \\
		T(\vec{e_4}) &= (1,-1,6)^T \\
	\end{aligned}
\]

As such we get the following matrix for this transformation:

\[A = \genericmat{p}{1&1&1&1\\0&1&0&-1\\1&3&0&6}\]

\subsection*{Part C}

$T: P_n \to P_n, Tf(t) = f'(t)$. Find this matrix with respect to the standard basis. 

Let $\beta = \left\{ 1, t, t^t, \cdots, t^n \right\}$.

\[
	\begin{aligned}
		T(1) = 0 &= (0,0,0, \dots , 0^T \\
			T(t) = 1 &= (1,0,0, \dots, 0)^T \\
			T(t^2) = 2t &= (0,2,0, \dots , 0)^T \\
			T(t^3) = 3t^2 &= (0,0,3, \dots,  0)^T \\
			T(t^n) = nt^{n-1} &= (0,0,0, \dots,  n)^T 
	\end{aligned}
\]

So,

\[
	A = \genericmat{p}{
		0&1&0&0& \dots & 0 \\
		0&0&2&0& \dots & 0 \\
		0&0&0&3& \dots & 0 \\
		\vdots & \vdots & \vdots & \vdots & \dots & \vdots \\
		0&0&0&0& \dots & n \\
	}
\]

\subsection*{Part D}
\[T: P_n \to P_n,\; Tf(t) = 2f(t) + 3f \myprime (t) - 4f \mydprime (t)\]

Let $\beta = \left\{ 1, t, t^t, \cdots, t^n \right\}$.

\[
	\begin{aligned}
		T(1) &= 2 \cdot 1 = 1 = \boxed{(1,0,0)^T} \\
		T(t) &= 2t + 3(1) = 2t + 3 = \boxed{(3,2,0)^T} \\
		T(t^2) &= 2t^2 + 6t - 24 = \boxed{(-24,6,2)^T} \\
		T(t^n) &= 2t^n + 3nt^{n-1} - 4(n^2-n)t^{n-2} = \boxed{(-4(n^2-2),3n,2)^T} \\
	\end{aligned}
\]

\[
A = 
\genericmat{p}
{
	2&3&-24&\dots&-4(n^2-n)\\
	0&2&6&\dots&3n\\
	0&0&2&\dots&2
}
\]
